modified:   c/cs/clean.sh 	new file:   c/cs/syscall/error.c 	new file:   c/cs/syscall/error.h 	new file:   c/cs/syscall/fork2.c 	new file:   c/cs/syscall/pause.c 	new file:   c/cs/syscall/sleep.c 	new file:   c/cs/syscall/waitpid.c 	new file:   c/cs/syscall/waitpid2.c 	modified:   coq/cat/Category6.v 	modified:   coq/cat/Eq.v 	modified:   coq/cat/Setoids.v 	new file:   coq/sf/Imp_code.v 	modified:   coq/sf/evalR.v 	copied:     coq/sf/evalR.v -> coq/sf/evalR_old.v 	modified:   coq/sf/syntax.v 	modified:   coq/sf/test_optimize.v 	new file:   haskell/ConsoleANSI.hs 	new file:   haskell/representable.hs 	new file:   haskell/wiwik/Haskeline.hs 	new file:   haskell/wiwik/Pretty.hs 	new file:   haskell/wiwik/Quasiquotation.hs 	new file:   haskell/wiwik/Repline.hs 	new file:   python/bitcoin/clightning.py 	new file:   python/bitcoin/lightning_test.py 	new file:   shell/node.sh 	new file:   shell/raspnode.sh

c/cs/syscall/error.c
@@ -1,0 +1,26 @@
+#include <stdio.h>
+#include <stdlib.h>
+#include <errno.h>
+#include <string.h>
+#include <unistd.h>
+
+
+#include "error.h"
+
+void unix_error(const char *msg)
+{   
+    fprintf(stderr, "%s: %s\n", msg, strerror(errno));
+    exit(0);
+} 
+
+pid_t Fork(void)
+{
+    pid_t pid;
+
+    if((pid = fork()) < 0)
+        unix_error("Fork error");
+
+    return pid;
+}
+
+
