c/cs/syscall/error.h
@@ -1,0 +1,5 @@
+#ifndef ERROR_INCLUDE_H
+#define ERROR_INCLUDE_H
+void unix_error(const char* msg);
+pid_t Fork(void);
+#endif
