c/cs/syscall/fork2.c
@@ -1,0 +1,34 @@
+#include <stdio.h>
+#include <stdlib.h>     /* exit     */
+#include <unistd.h>     /* fork     */
+#include <sys/wait.h>   /* waitpid  */ 
+
+/* we do not know whether parent or child will print first.
+ * possible outputs are :
+ *
+ * acbc
+ * abcc
+ * bacc
+ *
+ * But don't forget to flush stdout (or fprintf to stderr)
+ * Also, in practice, 'bacc' will dominate. Need to insert some 'sleep(1)' 
+ * in key points to see the other two possible outcome.
+ */
+
+int main ()
+{
+    if (fork() == 0) {
+        printf("a");
+        fflush(stdout);
+    }
+    else {
+        printf("b");
+        fflush(stdout);
+        waitpid(-1,NULL,0);
+    }
+    printf("c");
+    fflush(stdout);
+    exit(0);
+}
+
+
