c/cs/syscall/pause.c
@@ -1,0 +1,9 @@
+#include <unistd.h>
+
+int main() 
+{
+    int i;
+    i = pause(); /* need signal after that */
+
+    return 0;
+}
