c/cs/syscall/sleep.c
@@ -1,0 +1,15 @@
+#include <stdio.h>
+#include <unistd.h>
+
+
+int main()
+{
+
+    int i, sec = 5;
+
+    printf("sleeping for %d seconds\n", sec);
+    i = sleep(sec);
+    printf("return value is %d\n", i);
+
+    return 0;
+}
