c/cs/syscall/waitpid.c
@@ -1,0 +1,37 @@
+#include <stdio.h>
+#include <stdlib.h>
+#include <unistd.h>
+#include <sys/wait.h>
+#include <errno.h>
+
+#include "error.h"
+
+#define N 10
+
+
+int main()
+{
+
+    int status, i;
+    pid_t pid;
+
+    /* Parent creates N children */
+    for(i = 0; i < N; ++i)
+        if ((pid = Fork()) == 0) /* child */
+            exit (100 + i);
+
+    /* Parent reaps N children in no particuler order */
+    while ((pid = waitpid(-1,&status,0)) > 0) {
+        if(WIFEXITED(status))
+            printf("child %d terminated normally with exit status %d\n",
+                    pid, WEXITSTATUS(status));
+        else
+            printf("child %d terminated abnormally\n", pid);
+    }
+
+    /* The only normal termination is if there are no more children */
+    if(errno != ECHILD)
+        unix_error("waitpid error");
+
+    exit(0);
+}
