haskell/ConsoleANSI.hs
@@ -1,0 +1,12 @@
+import System.Console.ANSI
+
+-- works but colors are often not what you expect, just like with bash
+-- guessing terminal does not comply with standard
+
+main :: IO ()
+main = do
+--    setSGR [SetColor Foreground Dull Blue]
+    setSGR [SetColor Background Dull Red]
+    putStrLn "Red-On-Blue"
+    setSGR [Reset]
+    putStrLn "Default colors"
