haskell/representable.hs
@@ -1,0 +1,58 @@
+{-# LANGUAGE ExplicitForAll #-}
+{-# LANGUAGE DeriveFunctor #-}
+{-# LANGUAGE TypeFamilies #-}
+
+data F a = MkF { unF :: a} deriving (Functor, Eq)
+
+data A = A
+data B = B deriving Eq
+
+alpha :: forall x . (String -> x ) -> F x 
+alpha = undefined
+
+
+alpha' :: (String -> x ) -> F x 
+alpha' = undefined
+
+f :: A -> B
+f A = B
+
+f1 = fmap f . alpha
+f2 = alpha . fmap f
+
+h :: String -> A
+h _ = A
+
+g1 = fmap f (alpha h)
+g2 = alpha (f . h)
+
+beta :: forall x . F x -> (String -> x)
+beta = undefined
+
+
+-- The list functor is not representable
+
+gamma :: forall x. (Int -> x) -> [x]
+gamma h = map h [12]
+
+gamma_inverse :: forall x. [x] -> (Int -> x)
+gamma_inverse  = undefined -- cant do it 
+
+
+class Representable f where
+    type Rep f :: *   -- the 'a' in the natural isomorphism C(a,-) => f
+    tabulate   :: forall x. (Rep f -> x) -> f x
+    index      :: forall x. f x -> Rep f -> x 
+
+
+data Stream a = Cons a (Stream a)
+
+instance Representable Stream where
+    type Rep Stream = Integer
+    tabulate f = Cons (f 0) (tabulate (f . (+1)))
+    index (Cons b bs) n = if n == 0 then b else index bs (n - 1)
+
+
+
+
+
