haskell/wiwik/Haskeline.hs
@@ -1,0 +1,19 @@
+import Control.Monad.Trans
+import System.Console.Haskeline
+
+
+type Repl a = InputT IO a
+
+process :: String -> IO ()
+process = putStrLn
+
+repl :: Repl ()
+repl = do
+    minput <- getInputLine "Repl> "
+    case minput of
+        Nothing -> outputStrLn "Goodbye."
+        Just input -> (liftIO $ process input) >> repl
+
+
+main :: IO ()
+main = runInputT defaultSettings repl
