haskell/wiwik/Pretty.hs
@@ -1,0 +1,81 @@
+{-# LANGUAGE FlexibleInstances #-}
+
+import Text.PrettyPrint
+import Text.Show.Pretty (ppShow)
+
+parensIf :: Bool -> Doc -> Doc
+parensIf True   = parens
+parensIf False  = id
+
+type Name = String
+
+data Expr 
+    = Var String
+    | Lit Ground
+    | App Expr Expr
+    | Lam Name Expr
+    deriving (Eq,Show)
+
+
+data Ground 
+    = LInt Int
+    | LBool Bool
+    deriving (Eq,Show,Ord)
+
+
+class Pretty p where
+    ppr :: Int -> p -> Doc
+
+instance Pretty String where
+    ppr _ x = text x
+
+instance Pretty Expr where
+    ppr _ (Var x)           = text x
+    ppr _ (Lit (LInt a))    = text (show a)
+    ppr _ (Lit (LBool b))   = text (show b)
+    
+    ppr p e@(App _ _) =
+        let (f,xs) = viewApp e in 
+        let args = sep $ map (ppr (p+1)) xs in
+        parensIf (p>0) $ ppr p f <+> args
+
+    ppr p e@(Lam _ _) =
+        let body = ppr (p+1) (viewBody e) in
+        let vars = map (ppr 0) (viewVars e) in
+        parensIf (p>0) $ char '\\' <> hsep vars <+> text "." <+> body
+
+
+viewVars :: Expr -> [Name]
+viewVars (Lam n a) = n : viewVars a
+viewVars _ = []
+
+viewBody :: Expr -> Expr
+viewBody (Lam _ a) = viewBody a
+viewBody x = x
+
+
+viewApp :: Expr -> (Expr, [Expr])
+viewApp (App e1 e2) = go e1 [e2] where
+    go (App a b) xs = go a (b:xs)
+    go f xs = (f,xs)
+
+ppexpr :: Expr -> String
+ppexpr = render . ppr 0
+
+s,k, example :: Expr
+s = Lam "f" (Lam "g" (Lam "x" (App (Var "f") (App (Var "g") (Var "x")))))
+k = Lam "x" (Lam "y" (Var "x"))
+example = App s k
+
+main :: IO ()
+main = do
+    putStrLn $ ppexpr s
+    putStrLn $ ppShow example
+
+
+
+
+    
+
+
+
