haskell/wiwik/Quasiquotation.hs
@@ -1,0 +1,39 @@
+{-# LANGUAGE TemplateHaskell #-}
+
+import Control.Monad.Identity
+
+import Language.Haskell.TH.Syntax
+
+import Text.Parsec
+import Text.Parsec.String (Parser)
+import Text.Parsec.Language (emptyDef)
+
+import qualified Text.Parsec.Expr as Ex
+import qualified Text.Parsec.Token as Tok
+
+data Expr 
+    = Tr
+    | Fl
+    | Zero
+    | Succ Expr
+    | Pred Expr
+    deriving (Eq,Show)
+
+instance Lift Expr where
+    lift Tr         = [| Tr |]
+    lift Fl         = [| Fl |]
+    lift Zero       = [| Zero |]
+    lift (Succ a)   = [| Succ a |]
+    lift (Pred a)   = [| Pred a |]
+
+type Op = Ex.Operator String () Identity
+
+lexer :: Tok.TokenParser ()
+lexer = Tok.makeTokenParser emptyDef
+
+parens :: Parser a -> Parser a
+parens = Tok.parens lexer
+
+reserved :: String -> Parser ()
+reserved = Tok.reserved lexer
+
