haskell/wiwik/Repline.hs
@@ -1,0 +1,43 @@
+import Data.List (isPrefixOf)
+import System.Process (callCommand)
+import Control.Monad.Trans
+import System.Console.Repline
+
+
+type Repl a = HaskelineT IO a
+
+-- Evaluation : handle each line user inputs
+cmd :: String -> Repl ()
+cmd input = liftIO $ print input
+
+
+-- Tab completion : return a completion for parial words entered
+completer :: Monad m => WordCompleter m
+completer n = do
+    let names = ["kirk","spock","mccoy"]
+    return $ filter (isPrefixOf n) names
+
+-- Commands
+help :: [String] -> Repl ()
+help args = liftIO $ print $ "Help: " ++ show args
+
+
+say :: [String] -> Repl ()
+say args = do
+    _ <- liftIO $ callCommand $ "cowsay" ++ " " ++ (unwords args)
+    return ()
+
+options :: [(String,[String] -> Repl ())]
+options = [ ("help",help) , ("say", say) ]
+
+
+ini :: Repl ()
+ini = liftIO $ putStrLn "Welcome!"
+
+repl :: IO ()
+repl = evalRepl ">>> " cmd options (Word0 completer) ini
+
+main :: IO ()
+main = repl
+
+
