python/bitcoin/clightning.py
@@ -1,0 +1,55 @@
+import os
+import sys
+import logging
+import tempfile
+
+
+import utils  # PYTHONPATH set to /home/john/Libs/lightning/tests
+
+bitcoind = None
+TEST_DIR = tempfile.mkdtemp(prefix='lightning-')
+VALGRIND = os.getenv("NO_VALGRIND","0") == "0"
+DEVELOPER = os.getenv("DEVELOPER","0") == "1"
+TEST_DEBUG = os.getenv("TEST_DEBUG","0") == "1"
+
+
+print("Testing results are in {}".format(TEST_DIR))
+
+
+if TEST_DEBUG:
+    logging.basicConfig(level=logging.DEBUG, stream=sys.stderr)
+
+logging.info("Tests running in '%s'",TEST_DIR)
+
+
+# bitcoind testnet should be running
+bitcoind = utils.BitcoinD(bitcoin_dir="/home/john/.bitcoin/testnet3")
+
+info = bitcoind.rpc.getnetworkinfo()
+
+version = info['version']
+
+print(version)
+
+info = bitcoind.rpc.getblockchaininfo()
+
+blocks = info['blocks']
+
+print(blocks)
+
+info = bitcoind.rpc.getwalletinfo()
+
+balance = info['balance']
+print(balance)
+
+print(bitcoind.rpc.getblockcount())
+
+
+os.rmdir(TEST_DIR)
+
+
+
+
+
+
+
