python/bitcoin/lightning_test.py
@@ -1,0 +1,12 @@
+from lightning import LightningRpc
+import random
+
+l = LightningRpc("/home/john/.lightning/lightning-rpc")
+
+#invoice = l.invoice(100,"lbl{}".format(random.random()),"testpayment")
+
+route = l.getroute(l.getinfo()['id'],100,1)
+
+print(route)
+
+
