coq/cat/Category6.v
@@ -7,12 +7,15 @@ Record Category : Type := category
     ; id            : forall (a:Obj), Hom a a
     ; eqHom         : forall (a b:Obj), Eq (Hom a b)
     ; proof_idl     : forall (a b:Obj) (f:Hom a b), 
-        eq (eqHom a b) (compose _ _ _ (id b) f) f
+        equal (eqHom a b) (compose _ _ _ (id b) f) f
     ; proof_idr     : forall (a b:Obj) (f:Hom a b),
-        eq (eqHom a b) (compose _ _ _ f (id a)) f 
+        equal (eqHom a b) (compose _ _ _ f (id a)) f 
     ; proof_assoc   : forall (a b c d:Obj)(f:Hom a b)(g:Hom b c)(h:Hom c d),
-        eq (eqHom a d)  (compose _ _ _ h (compose _ _ _ g f))
-                        (compose _ _ _ (compose _ _ _ h g) f)
+        equal (eqHom a d) (compose _ _ _ h (compose _ _ _ g f))
+                          (compose _ _ _ (compose _ _ _ h g) f)
+    ; proof_compat  : forall (a b c:Obj) (f f':Hom a b) (g g':Hom b c),
+        equal (eqHom a b) f f' -> equal (eqHom b c) g g' -> 
+        equal (eqHom a c) (compose _ _ _ g f) (compose _ _ _ g' f')
     }
     .
 
@@ -23,10 +26,11 @@ Arguments eqHom {c} {a} {b}.
 Arguments proof_idl {c} {a} {b} _.
 Arguments proof_idr {c} {a} {b} _.
 Arguments proof_assoc {c} {a} {b} {c0} {d} _ _ _.
+Arguments proof_assoc {c} {a} {b} {c0} _ _ _ _.
 
 Notation "g @ f" := (compose g f) (at level 60, right associativity). 
 
-Notation "f == g" := (eq eqHom f g) (at level 90, no associativity).
+Notation "f == g" := (equal eqHom f g) (at level 90, no associativity).
 
 Lemma id_left : forall (C:Category) (a b:Obj C) (f:Hom a b), (id b) @ f == f.
 Proof. intros C a b f. apply proof_idl. Qed.
@@ -37,4 +41,8 @@ Proof. intros C a b f. apply proof_idr. Qed.
 Lemma assoc : forall (C:Category)(a b c d:Obj C)(f:Hom a b)(g:Hom b c)(h:Hom c d), 
     h @ (g @ f) == (h @ g) @ f.
 Proof. intros C a b c d f g h. apply proof_assoc. Qed.
+
+Lemma compat : forall (C:Category)(a b c:Obj C)(f f':Hom a b)(g g':Hom b c),
+    f == f' -> g == g' -> g @ f == g' @ f'.
+Proof. intros C a b c f f' g g'. apply proof_compat. Qed.
 
