coq/sf/evalR.v
@@ -2,81 +2,90 @@ Require Import nat.
 Require Import bool.
 Require Import syntax.
 Require Import eval.
+Require Import state.
 
-(*
 
-Reserved Notation "e 'a=>' n" (at level 90, no associativity).
+Inductive aevalR:State -> aexp -> nat -> Prop :=
+| E_ANum  : forall e n, aevalR e (ANum n) n
+| E_AKey  : forall e k, aevalR e (AKey k) (e k)
+| E_APlus : forall e n1 n2 a1 a2, 
+    aevalR e a1 n1 -> aevalR e a2 n2 -> aevalR e (APlus  a1 a2) (n1 + n2)
+| E_AMinus: forall e n1 n2 a1 a2, 
+    aevalR e a1 n1 -> aevalR e a2 n2 -> aevalR e (AMinus a1 a2) (n1 - n2)
+| E_AMult : forall e n1 n2 a1 a2, 
+    aevalR e a1 n1 -> aevalR e a2 n2 -> aevalR e (AMult  a1 a2) (n1 * n2)
+.
 
-Inductive aevalR:aexp -> nat -> Prop :=
-| E_ANum  : forall n, (ANum n) a=> n
-| E_APlus : forall n1 n2 a1 a2, a1 a=> n1 -> a2 a=> n2 -> APlus  a1 a2 a=> n1 + n2
-| E_AMinus: forall n1 n2 a1 a2, a1 a=> n1 -> a2 a=> n2 -> AMinus a1 a2 a=> n1 - n2
-| E_AMult : forall n1 n2 a1 a2, a1 a=> n1 -> a2 a=> n2 -> AMult  a1 a2 a=> n1 * n2
+Inductive bevalR:State-> bexp -> bool -> Prop :=
+| E_BTrue : forall e, bevalR e BTrue true
+| E_BFalse: forall e, bevalR e BFalse false
+| E_BEq   : forall e n1 n2 a1 a2, 
+    aevalR e a1 n1 -> aevalR e a2 n2 -> bevalR e (BEq a1 a2) (eqb n1 n2) 
+| E_BLe   : forall e n1 n2 a1 a2, 
+    aevalR e a1 n1 -> aevalR e a2 n2 -> bevalR e (BLe a1 a2) (leb n1 n2)
+| E_BNot  : forall e b1 e1, 
+    bevalR e e1 b1 -> bevalR e (BNot e1) (negb b1)
+| E_BAnd  : forall e b1 b2 e1 e2,
+    bevalR e e1 b1 -> bevalR e e2 b2 -> bevalR e (BAnd e1 e2) (andb b1 b2) 
+.
 
-where "e 'a=>' n" := (aevalR e n).
-
-Reserved Notation "e 'b=>' b" (at level 90, no associativity).
-
-Inductive bevalR:bexp -> bool -> Prop :=
-| E_BTrue : BTrue   b=> true
-| E_BFalse: BFalse  b=> false
-| E_BEq   : forall n1 n2 a1 a2, a1 a=> n1 -> a2 a=> n2 -> BEq a1 a2 b=> eqb n1 n2 
-| E_BLe   : forall n1 n2 a1 a2, a1 a=> n1 -> a2 a=> n2 -> BLe a1 a2 b=> leb n1 n2 
-| E_BNot  : forall b1 e1, e1 b=> b1 -> BNot e1 b=> negb b1
-| E_BAnd  : forall b1 b2 e1 e2,e1 b=> b1 -> e2 b=> b2 -> BAnd e1 e2 b=> andb b1 b2 
-
-where "e 'b=>' b" := (bevalR e b).
-
-Theorem aeval_iff_aevalR : forall (a:aexp) (n:nat),
-    a a=> n <-> aeval a = n.
+Theorem aeval_iff_aevalR : forall (env:State) (a:aexp) (n:nat),
+    aevalR env a n <-> aeval env a = n.
 Proof.
-    intros a n. split.
+    intros env a n. split.
     - intro H. induction H as   [ n
-                                | n1 n2 a1 a2 H1 IH1 H2 IH2
-                                | n1 n2 a1 a2 H1 IH1 H2 IH2
-                                | n1 n2 a1 a2 H1 IH1 H2 IH2
+                                | k
+                                | e n1 n2 a1 a2 H1 IH1 H2 IH2
+                                | e n1 n2 a1 a2 H1 IH1 H2 IH2
+                                | e n1 n2 a1 a2 H1 IH1 H2 IH2
                                 ].
+        + reflexivity.
         + reflexivity.
         + simpl. rewrite IH1, IH2. reflexivity.
         + simpl. rewrite IH1, IH2. reflexivity.
         + simpl. rewrite IH1, IH2. reflexivity.
-    - revert n. induction a as [n|a1 H1 a2 H2| a1 H1 a2 H2| a1 H1 a2 H2].
-        + simpl. intros p H. subst. apply E_ANum.
-        + simpl. intros p H. subst. apply E_APlus. 
+
+    - revert n env. induction a as [n|k|a1 H1 a2 H2| a1 H1 a2 H2| a1 H1 a2 H2].
+        + simpl. intros p e H. subst. apply E_ANum.
+        + simpl. intros p e H. subst. apply E_AKey.
+        + simpl. intros p e H. subst. apply E_APlus. 
             { apply H1. reflexivity. }
             { apply H2. reflexivity. }
-        + simpl. intros p H. subst. apply E_AMinus. 
+        + simpl. intros p e H. subst. apply E_AMinus. 
             { apply H1. reflexivity. }
             { apply H2. reflexivity. }
-        + simpl. intros p H. subst. apply E_AMult. 
+        + simpl. intros p e H. subst. apply E_AMult. 
             { apply H1. reflexivity. }
             { apply H2. reflexivity. }
 Qed.
 
-
-Theorem aeval_iff_aevalR' : forall (a:aexp) (n:nat),
-    a a=> n <-> aeval a = n.
+Theorem aeval_iff_aevalR' : forall (env:State) (a:aexp) (n:nat),
+    aevalR env a n <-> aeval env a = n.
 Proof. 
     split. 
     - intros H. induction H; subst; reflexivity.
-    - revert n. induction a as [n|a1 H1 a2 H2| a1 H1 a2 H2| a1 H1 a2 H2]; 
+    - revert n env. induction a as [n|k|a1 H1 a2 H2| a1 H1 a2 H2| a1 H1 a2 H2]; 
         simpl; intros; subst; constructor; 
         try apply H1; try apply H2; reflexivity.  
 Qed.
 
-Theorem beval_iff_bevalR : forall (e:bexp) (b:bool),
-    e b=> b <-> beval e = b.
+
+Theorem beval_iff_bevalR : forall (env:State) (e:bexp) (b:bool),
+    bevalR env e b <-> beval env e = b.
 Proof.
     split.
     - intros H. induction H; subst; try reflexivity; simpl.
-        +  assert (aeval a1 = n1) as H1. { apply aeval_iff_aevalR. assumption. }
-           assert (aeval a2 = n2) as H2. { apply aeval_iff_aevalR. assumption. }
+        + assert (aeval e a1 = n1) as H1. 
+            { apply aeval_iff_aevalR. assumption. }
+          assert (aeval e a2 = n2) as H2. 
+            { apply aeval_iff_aevalR. assumption. }
            rewrite H1, H2. reflexivity.
-        +  assert (aeval a1 = n1) as H1. { apply aeval_iff_aevalR. assumption. }
-           assert (aeval a2 = n2) as H2. { apply aeval_iff_aevalR. assumption. }
+        +  assert (aeval e a1 = n1) as H1. 
+            { apply aeval_iff_aevalR. assumption. }
+           assert (aeval e a2 = n2) as H2. 
+               { apply aeval_iff_aevalR. assumption. }
            rewrite H1, H2. reflexivity.
     - revert b. induction e as [ | |a1 a2|a1 a2|e1 H1|e1 H1 e2 H2];
         intros; subst; simpl; constructor; try apply aeval_iff_aevalR; 
         try reflexivity; try apply H1; try apply H2; reflexivity.
 Qed.
-*)
