coq/sf/Imp_code.v
@@ -1,0 +1,26 @@
+Require Import nat.
+Require Import syntax.
+Require Import state.
+
+Definition fact_in_coq : com :=
+    z ::= AKey x;; 
+    y ::= ANum 1;;
+    WHILE BNot (BEq (AKey z) (ANum 0)) DO
+        y ::= AMult (AKey y) (AKey z);;
+        z ::= AMinus (AKey z) (ANum 1)
+    END.
+
+
+Definition Add2_x : com := x ::= (APlus (AKey x) (ANum 2)).
+
+Definition Mult_x_y_z : com := z::= AMult (AKey x) (AKey y).
+
+Definition Dec_x_z : com := 
+    z ::= AMinus (AKey z) (ANum 1);;
+    x ::= AMinus (AKey x) (ANum 1).
+
+
+
+
+ 
+
