coq/sf/syntax.v
@@ -18,3 +18,31 @@ Inductive bexp : Type :=
 | BNot   : bexp -> bexp
 | BAnd   : bexp -> bexp -> bexp
 .
+
+
+Inductive com : Type :=
+| CSkip  : com
+| CAss   : Key -> aexp -> com
+| CSeq   : com -> com -> com
+| CIf    : bexp -> com -> com -> com
+| CWhile : bexp -> com -> com
+.
+
+
+Notation "'SKIP'"    := CSkip.
+
+Notation "x '::=' a" := (CAss x a) 
+(at level 60).
+
+Notation "c1 ;; c2"  := (CSeq c1 c2) 
+(at level 80, right associativity). 
+
+Notation "'WHILE' b 'DO' c 'END'" := (CWhile b c) 
+(at level 80, right associativity).
+
+Notation "'IFB' b 'THEN' c1 'ELSE' c2 'FI'" := (CIf b c1 c2) 
+(at level 80, right associativity).
+
+
+
+
