coq/sf/test_optimize.v
@@ -5,7 +5,6 @@ Require Import eval.
 Require Import optimize.
 Require Import state.
 
-(*
 
 Theorem optimize_0plus_sound : forall (a:aexp) (env:State), 
     aeval env (optimize_0plus a) = aeval env a.
@@ -16,45 +15,44 @@ Proof.
     - simpl. intros env. destruct a1 as [[|n]|[n]|b1 b2|b1 b2|b1 b2].
         + simpl. rewrite IH2. reflexivity.
         + simpl. rewrite IH2. reflexivity.
+        + simpl. rewrite IH2. reflexivity.
         + simpl. simpl in IH1. rewrite IH1. rewrite IH2. reflexivity.
         + simpl. simpl in IH1. rewrite IH1. rewrite IH2. reflexivity.
         + simpl. simpl in IH1. rewrite IH1. rewrite IH2. reflexivity.
-    - simpl. rewrite IH1, IH2. reflexivity.
-    - simpl. rewrite IH1, IH2. reflexivity. 
+    - simpl. intros env. rewrite IH1, IH2. reflexivity.
+    - simpl. intros env. rewrite IH1, IH2. reflexivity. 
    
 Qed.
-*)  
 
 
-(*
-Theorem optimize_0plus_sound2 : forall (a:aexp), 
-    aeval (optimize_0plus a) = aeval a.
+Theorem optimize_0plus_sound2 : forall (a:aexp) (env:State), 
+    aeval env (optimize_0plus a) = aeval env a.
 Proof.
-    intros a. induction a as [n|a1 IH1 a2 IH2|a1 IH1 a2 IH2|a1 IH1 a2 IH2]. 
+    intros a. induction a as [n|k|a1 IH1 a2 IH2|a1 IH1 a2 IH2|a1 IH1 a2 IH2]. 
     - reflexivity.
-    - simpl. destruct a1 as [[|n]|b1 b2|b1 b2|b1 b2]; 
+    - reflexivity.
+    - simpl. intros env. destruct a1 as [[|n]|[n]|b1 b2|b1 b2|b1 b2]; 
         simpl; 
         simpl in IH1;
         try rewrite IH1;
         rewrite IH2;
         reflexivity.
-    - simpl. rewrite IH1, IH2. reflexivity.
-    - simpl. rewrite IH1, IH2. reflexivity. 
+    - simpl. intros env. rewrite IH1, IH2. reflexivity.
+    - simpl. intros env. rewrite IH1, IH2. reflexivity. 
 Qed.
 
-
-Theorem optimize_0plus_b_sound : forall (b:bexp),
-   beval (optimize_0plus_b b) = beval b.
+Theorem optimize_0plus_b_sound : forall (b:bexp) (env:State),
+   beval env (optimize_0plus_b b) = beval env b.
 Proof.
     intros b. induction b as [| |a1 a2|a1 a2|b1 IH1|b1 IH1 b2 IH2].
     - reflexivity.
     - reflexivity.
-    - simpl. rewrite (optimize_0plus_sound a1), (optimize_0plus_sound a2).
+    - simpl. intros env. 
+        rewrite (optimize_0plus_sound a1), (optimize_0plus_sound a2).
         reflexivity.
-    - simpl. rewrite (optimize_0plus_sound a1), (optimize_0plus_sound a2).
+    - simpl. intros env.
+        rewrite (optimize_0plus_sound a1), (optimize_0plus_sound a2).
         reflexivity.
-    - simpl. rewrite IH1. reflexivity.
-    - simpl. rewrite IH1, IH2. reflexivity.
+    - simpl. intros env. rewrite IH1. reflexivity.
+    - simpl. intros env. rewrite IH1, IH2. reflexivity.
 Qed.
-
-*)
