c/cs/clean.sh
@@ -13,6 +13,8 @@ rm -f *.o
 rm -f *.s
 rm -f gmon.out
 rm -f log
+rm -f *.lo
+rm -fr .libs 
 
 mv pushtest.ss pushtest.s
 
