shell/node.sh
@@ -1,0 +1,69 @@
+#!/bin/bash
+
+echo "node.sh starting"
+
+# (e)xit on error, treat (u)nset variable as error
+set -eu
+
+TEXT_RESET='\e[0m'
+TEXT_RED='\e[0;31m'
+TEXT_GREEN='\e[0;32m'
+TEXT_YELLOW='\e[0;33m'
+TEXT_BLUE='\e[0;34m'
+TEXT_MAGENTA='\e[0;35m' # between pink and purple
+TEXT_CYAN='\e[0;36m'    # light ugly blue
+TEXT_WHITE='\e[0;37m'
+TEXT_GREY='\e[0;38m'    # same as reset color it seems
+
+
+user=$(logname)
+PUBLICIP=$(curl icanhazip.com 2> /dev/null)
+
+function writeGreen(){
+    echo -e -n "${TEXT_GREEN}${1}"
+    echo -e -n "${TEXT_RESET}"
+}
+
+function writeYellow(){
+    echo -e -n "${TEXT_YELLOW}${1}"
+    echo -e -n "${TEXT_RESET}"
+}
+
+function writeRed(){
+    echo -e -n "${TEXT_RED}${1}"
+    echo -e -n "${TEXT_RESET}"
+}
+
+function writeBlue(){
+    echo -e -n "${TEXT_BLUE}${1}"
+    echo -e -n "${TEXT_RESET}"
+}
+
+function writeMagenta(){                # betwen pink and purple
+    echo -e -n "${TEXT_MAGENTA}${1}"
+    echo -e -n "${TEXT_RESET}"
+}
+
+function writeCyan(){
+    echo -e -n "${TEXT_CYAN}${1}"
+    echo -e -n "${TEXT_RESET}"
+}
+
+function writeWhite(){
+    echo -e -n "${TEXT_WHITE}${1}"
+    echo -e -n "${TEXT_RESET}"
+}
+
+function writeGrey(){
+    echo -e -n "${TEXT_GREY}${1}"
+    echo -e -n "${TEXT_RESET}"
+}
+
+TEXT_TRY='\e[1;41m'
+
+function writeTry(){
+    echo -e -n "${TEXT_TRY}${1}"
+    echo -e -n "${TEXT_RESET}"
+}
+
+echo "node.sh complete"
