shell/raspnode.sh
@@ -1,0 +1,306 @@
+#!/bin/bash
+##############################################################################################
+#
+# jochemin
+#
+#Bitcoin + Lightning node installation bash script
+#
+#Raspberry + external USB drive required, pendrive recommended
+#
+#BTC Donations. Thank you!! --> 3FM6FypcrSVhdHh7cpVQMrhPXPZ6zcXeYU
+#
+#LN 1000 satoshi --> lnbc10u1pdtyqucpp52fu993pgr4vx8kw7un53wc6nr2v979ca53wsr7swkaxaxewgep6qdqlgysxyet9wgsxvmmjyp4x7cmgv4kkjmscqzysxq92ptxs5jyam5u65rlfhrls2khe60lt93m2zyv06tzjkxt9u6l50jy63v7xu4pqah2kr3kljmhq8zyeaw02t3vcygde4nglm48fruk6x4lmf8gqueegmf
+#
+#Connect to my LN node --> 02d249db09237f974f1c67775accee37a9d1eb3f04f236dda177f5a5c083094f15@jocheminlnd1.ddns.net:9735
+##############################################################################################
+echo "wrong script !!!"
+exit 0
+
+# Fail on error , debug all lines#############################################################
+set -eu -o pipefail
+##############################################################################################
+
+
+#Some color for text#########################################################################
+TEXT_RESET='\e[0m'
+TEXT_YELLOW='\e[0;33m'
+TEXT_RED_B='\e[1;31m'
+#TEXT_GREEN='\e[0;32m'
+##############################################################################################
+
+# variables###################################################################################
+user=$(logname)
+userhome='/home/'$user
+FOLD1='/dev/'
+PUBLICIP="$(curl ipinfo.io/ip)"
+##############################################################################################
+
+# Color functions#############################################################################
+function writegreen(){
+    echo -e -n "'\e[0;32m$1"
+    echo -e -n '\033[0m\n'
+}
+function writeyellow(){
+    echo -e -n "'\e[0;33m$1"
+    echo -e -n '\033[0m\n'
+}
+function writered(){
+    echo -e -n "'\e[1;31m$1"
+    echo -e -n '\033[0m\n'
+}
+##############################################################################################
+
+# External HD detection and prompt for format#################################################
+function hd_detect {
+    drive_find="$(lsblk -dlnb | awk '$4>=193273528320' | numfmt --to=iec --field=4 | cut -c1-3)"
+    drive=$FOLD1$drive_find
+    drive_size="$(df -h "$drive" | sed 1d |  awk '{print $2}')"
+    while true; do
+        echo -e "$TEXT_RED_B"
+        read -p "$drive_size $drive will be formatted. Are you agree? (y/n) " yn
+        case $yn in
+            [Yy]* ) DRIVE_CONF=true;break;;
+            [Nn]* ) echo "This script needs to format an entire hard disk.";echo -e "$TEXT_RESET";exit;;
+            * ) echo "Please answer yes or no. (y/n)";;
+        esac
+        echo -e "$TEXT_RESET"
+    done
+}
+##############################################################################################
+
+
+# HD configuration############################################################################
+function hd_conf {
+    drive=$drive"1"
+    if mount | grep "$drive" > /dev/null;then
+        umount -l "$drive" > /dev/null
+    fi
+    writeyellow 'Formatting hard disk'
+    sudo mkfs.ext4 -F "$drive" -L BITCOIN
+    writegreen 'Hard disk formatted'
+    UUID="$(blkid -o value -s UUID "$drive")"
+    writeyellow 'Creating Bitcoin data folder'
+    BTCDIR='/home/'$user'/.bitcoin'
+    mkdir -p "$BTCDIR"
+    writeyellow 'Modifying fstab'
+    sudo sed -i".bak" "/$UUID/d" /etc/fstab
+    echo "UUID=$UUID  $BTCDIR  ext4  defaults,noatime  0    0" >> /etc/fstab
+    if mount | grep "$drive" > /dev/null;then
+        :
+    else
+        sudo mount -a
+    fi
+    sudo chmod 777 "$BTCDIR"
+    writegreen 'Hard disk configured'
+}
+##############################################################################################
+
+# CONFIGURE SWAP IN THE HARD DRIVE############################################################
+function swap_conf {
+    writeyellow 'Configuring swap in the hard drive'
+    sudo -u "$user" mkdir -p /home/"$user"/.bitcoin/swap
+    dd if=/dev/zero of=/home/"$user"/.bitcoin/swap/swap.file bs=1M count=2148
+    chmod 600 /home/"$user"/.bitcoin/swap/swap.file
+    sudo sed -i".bak" "/CONF_SWAPFILE/d" /etc/dphys-swapfile
+    sudo sed -i".bak" "/CONF_SWAPSIZE/d" /etc/dphys-swapfile
+    echo "CONF_SWAPFILE=/home/$user/.bitcoin/swap/swap.file" >> /etc/dphys-swapfile
+    echo "CONF_SWAPSIZE=2048" >> /etc/dphys-swapfile
+    mkswap /home/"$user"/.bitcoin/swap/swap.file
+    swapon /home/"$user"/.bitcoin/swap/swap.file
+    echo "/home/$user/.bitcoin/swap/swap.file  none  swap  defaults  0    0" >> /etc/fstab
+    writegreen 'swap configured'
+}
+# USER INPUT##################################################################################
+function user_input {
+    # Do we have an external hard drive?
+    while true; do
+        echo -e "$TEXT_YELLOW"
+        read -p "Is the hard drive connected? It will be formated. (y/n)" yn
+        case $yn in
+            [Yy]* ) hd_detect;break;; #If we have HD_CONFIG value says to configure it.
+            [Nn]* ) echo "Please connect an USB hard drive an retry";exit;;
+            * ) echo "Please answer yes or no. (y/n)";;
+        esac
+    done
+    echo 'Bitcoin and LND need a RPC user and password, please insert data.'
+    read -p 'Insert username: ' rpcuser
+    read -s -p 'Insert password: (will not be shown) ' rpcpass
+    echo 
+    read -p 'Insert your LND node alias: ' LNALIAS
+    echo -e "$TEXT_RESET"
+    # Do we have a pendrive for SWAP? IMPROVEMENT?
+    #while true; do
+    #    echo -e $TEXT_YELLOW
+    #    read -p "Will you use a pendrive for SWAP?" yn
+    #    case $yn in
+    #        [Yy]* ) SWAP_CONFIG=pen;break;; #If we have SWAP_CONFIG value says to configure it.
+    #        [Nn]* ) echo "SWAP will be set on external Hard Disk";SWAP_CONFIG=hd;break;; #else we configure swap in the external hard drive.
+    #        * ) echo "Please answer yes or no.";;
+    #    esac
+    #    echo -e $TEXT_RESET
+    #done
+}
+##############################################################################################
+
+# UPDATE RASPBERRY ###########################################################################
+function update_rasp {
+    writeyellow 'Updating Raspberry'
+    sudo apt-get update
+    writegreen 'APT update finished...'
+    sudo apt-get -y dist-upgrade
+    writegreen 'APT distributive upgrade finished...'
+    sudo apt-get -y upgrade
+    writegreen 'APT upgrade finished...'
+    sudo apt-get -y autoremove
+    writegreen 'APT auto remove finished...'
+
+    if [ -f /var/run/reboot-required ]; then
+        writered 'Reboot required!'
+    fi
+}
+##############################################################################################
+
+# INSTALL BERKELEY (4.8.30)###################################################################
+function install_berkeley {
+    writeyellow 'Installing database...'
+    sudo -u "$user" mkdir -p "$userhome"/bin
+    cd "$userhome"/bin
+    sudo -u "$user" wget http://download.oracle.com/berkeley-db/db-4.8.30.NC.tar.gz
+    sudo -u "$user" tar -xzvf db-4.8.30.NC.tar.gz
+    cd db-4.8.30.NC/build_unix/
+    ../dist/configure --enable-cxx
+    make
+    sudo make install
+    writegreen 'Database installed'
+}
+##############################################################################################
+
+# INSTALL BITCOIN CORE #######################################################################
+function install_bitcoin_core {
+    writeyellow 'Installing Bitcoin Core'
+    rm -fR "$userhome"/bin/bitcoin
+    cd "$userhome"/bin
+    git clone -b 0.16 https://github.com/bitcoin/bitcoin.git
+    cd bitcoin/
+    ./autogen.sh
+    ./configure CPPFLAGS="-I/usr/local/BerkeleyDB.4.8/include -O2" LDFLAGS="-L/usr/local/BerkeleyDB.4.8/lib" --enable-upnp-default
+    make
+    sudo make install
+    writegreen 'Bitcoin Core Installed'
+}
+##############################################################################################
+
+# BUILD BITCOIN.CONF##########################################################################
+function build_bitcoinconf {
+    echo 'zmqpubrawblock=tcp://127.0.0.1:18501' > /home/"$user"/.bitcoin/bitcoin.conf
+    echo 'zmqpubrawtx=tcp://127.0.0.1:18501' >> /home/"$user"/.bitcoin/bitcoin.conf
+    echo "rpcuser=$rpcuser" >> /home/"$user"/.bitcoin/bitcoin.conf
+    echo "rpcpassword=$rpcpass" >> /home/"$user"/.bitcoin/bitcoin.conf
+    echo 'dbcache=100' >> /home/"$user"/.bitcoin/bitcoin.conf
+    echo 'maxmempool=100' >> /home/"$user"/.bitcoin/bitcoin.conf
+    echo 'usehd=1' >> /home/"$user"/.bitcoin/bitcoin.conf
+    echo 'txindex=1' >> /home/"$user"/.bitcoin/bitcoin.conf
+    echo 'daemon=1' >> /home/"$user"/.bitcoin/bitcoin.conf
+    echo 'server=1' >> /home/"$user"/.bitcoin/bitcoin.conf
+}
+##############################################################################################
+
+# INSTALL LND#################################################################################
+function install_lnd {
+    writeyellow 'Installing LND 0.4 BETA'
+    cd "$userhome"
+    sudo -u "$user" mkdir -p download
+    cd download
+    wget https://github.com/lightningnetwork/lnd/releases/download/v0.4-beta/lnd-linux-arm-v0.4-beta.tar.gz
+    tar -xzf lnd-linux-arm-v0.4-beta.tar.gz
+    sudo install -m 0755 -o root -g root -t /usr/local/bin lnd-linux-arm-v0.4-beta/*
+}
+##############################################################################################
+
+# BUILD LND CONFIG FILE#######################################################################
+function build_lndconf {
+    sudo -u "$user" mkdir -p "$userhome"/.lnd
+    echo 'bitcoin.active=1' > "$userhome"/.lnd/lnd.conf
+    echo "externalip=$PUBLICIP" >> "$userhome"/.lnd/lnd.conf
+    echo "alias=$LNALIAS" >> "$userhome"/.lnd/lnd.conf
+    echo 'color=#1d8c09' >> "$userhome"/.lnd/lnd.conf
+    echo 'bitcoin.node=bitcoind' >> "$userhome"/.lnd/lnd.conf
+    echo "bitcoind.rpcuser=$rpcuser" >> "$userhome"/.lnd/lnd.conf
+    echo "bitcoind.rpcpass=$rpcpass" >> "$userhome"/.lnd/lnd.conf
+    echo 'bitcoind.zmqpath=tcp://127.0.0.1:18501' >> "$userhome"/.lnd/lnd.conf
+    #autopilot.active=1 >> $userhome/.lnd/lnd.conf
+    #autopilot.maxchannels=5 >> $userhome/.lnd/lnd.conf
+    #autopilot.allocation=0.6 >> $userhome/.lnd/lnd.conf
+}
+##############################################################################################
+
+# INSTALL PREREQUISITES#######################################################################
+function install_prerequisites {
+    writeyellow 'Installing prerequisites'
+    sudo apt-get install -y autoconf automake build-essential git libtool libevent-dev libgmp-dev libsqlite3-dev python python3 net-tools libboost-system-dev libboost-filesystem-dev libboost-chrono-dev libboost-program-options-dev libboost-test-dev libboost-thread-dev libssl-dev tmux
+    writegreen 'Prerequisites installed'
+}
+# MAIN - MAIN - MAIN - MAIN - MAIN - MAIN - MAIN - MAIN - MAIN - MAIN - MAIN - MAIN - MAIN ###
+# Check if script is launched with sudo#######################################################
+if [ "$(id -u)" -ne 0 ]; then
+    writered "Please run this script with sudo" >&2
+    exit 1
+fi
+##############################################################################################
+
+# Clean the screen############################################################################
+clear
+##############################################################################################
+
+# User input##################################################################################
+user_input
+##############################################################################################
+
+# Prerequisites###############################################################################
+writegreen 'Script will begin the installation, take a rest.'
+writegreen '____________________________________________________'
+update_rasp
+install_prerequisites
+##############################################################################################
+
+# Configure external hard drive###############################################################
+if [ "$DRIVE_CONF" = "true" ]; then
+    hd_conf
+    swap_conf
+fi
+##############################################################################################
+
+# INSTALL DATABASE (BERKELEY 4.8.30)##########################################################
+install_berkeley
+##############################################################################################
+
+# INSTALL BITCOIN CORE #######################################################################
+install_bitcoin_core
+build_bitcoinconf
+##############################################################################################
+
+#INSTALL LND##################################################################################
+install_lnd
+build_lndconf
+##############################################################################################
+
+# START BITCOIND##############################################################################
+writeyellow 'Starting Bitcoin Core'
+sudo -u "$user" bitcoind &
+writegreen 'Bitcoin Core started'
+##############################################################################################
+
+# START LND ##################################################################################
+# Wait 20 minutes for bitcoind to warm up
+writeyellow 'Waiting 20 minutes to start LND'
+sleep 20m
+sudo -u "$user" tmux new-session -d -s LND
+sudo -u "$user" tmux send-keys -t LND "lnd --bitcoin.mainnet" Enter
+writegreen 'LND started in tmux session'
+##############################################################################################
+
+#THE END #####################################################################################
+writegreen 'Please create a new Lightning wallet with lncli create.'
+writegreen 'To enter LND tmux session --> tmux a LND'
+writegreen 'Now you have to wait until syncing. Patience.'
+# MAIN - MAIN - MAIN - MAIN - MAIN - MAIN - MAIN - MAIN - MAIN - MAIN - MAIN - MAIN - MAIN ###
